Added the simple fork rewrite + sample Dynamatic Dot + changed mod field

DataflowRewriter/Rewrites/ForkRewrite.lean
@@ -7,7 +7,7 @@ Authors: Yann Herklotz
 import DataflowRewriter.Rewriter
 import DataflowRewriter.ExprHighElaborator
 
-namespace DataflowRewriter.MergeRewrite
+namespace DataflowRewriter.ForkRewrite
 
 /--
 The matcher takes in a dot graph and should return the cluster of nodes that
@@ -16,90 +16,90 @@ form the subgraph as a list of instance names.
 def matcher (g : ExprHigh String) : RewriteResult (List String) := do
   let (.some list) ← g.modules.foldlM (λ nodes inst (pmap, typ) => do
       if nodes.isSome then return nodes
-      unless typ = "Merge" do return none
-      let (.some nn) := followOutput g inst "out0" | return none
-      unless nn.typ = "Merge" && nn.inputPort = "inp0" do return none
+      unless typ = "Fork" do return none
+      let (.some nn) := followOutput g inst "out1" | return none
+      unless nn.typ = "Fork" && nn.inputPort = "inp0" do return none
       return some [inst, nn.inst]
     ) none | throw .done
   return list
 
-@[drunfold] def mergeLhs : ExprHigh String := [graph|
+@[drunfold] def Lhs : ExprHigh String := [graph|
     out0 [type = "io"];
+    out1 [type = "io"];
+    out2 [type = "io"];
     inp0 [type = "io"];
-    inp1 [type = "io"];
-    inp2 [type = "io"];
 
-    merge1 [type = "Merge"];
-    merge2 [type = "Merge"];
+    fork1 [type = "Fork"];
+    fork2 [type = "Fork"];
 
-    inp0 -> merge1 [inp = "inp0"];
-    inp1 -> merge1 [inp = "inp1"];
-    inp2 -> merge2 [inp = "inp1"];
+    inp0 -> fork1 [inp = "inp0"];
 
-    merge1 -> merge2 [out = "out0", inp = "inp0"];
+    fork1 -> out0 [out = "out0"];
+    fork1 -> fork2 [out = "out1", inp = "inp0"];
 
-    merge2 -> out0 [out = "out0"];
+    fork2 -> out1 [out = "out0"];
+    fork2 -> out2 [out = "out1"];
   ]
 
 /--
 To get instances in a predictable order, it's a good idea to extract the whole
 graph once with the nodes in the order that you want to provide them in the
-pattern-matcher.  In this case we want merge1 to be listed before merge2.
+pattern-matcher.  In this case we want fork1 to be listed before fork2.
 -/
-def mergeLhsOrdered := mergeLhs.extract ["merge1", "merge2"] |>.get rfl
+def LhsOrdered := Lhs.extract ["fork1", "fork2"] |>.get rfl
 
 /--
 Graph extraction gives back two graphs, the subgraph and the rest of the graph.
 Here we just double check that the rest of the graph is empty, implying we
 extracted the whole graph.  The proof of `rfl` should always work for this.
 -/
-theorem double_check_empty_snd : mergeLhsOrdered.snd = ExprHigh.mk ∅ ∅ := by rfl
+theorem double_check_empty_snd : LhsOrdered.snd = ExprHigh.mk ∅ ∅ := by rfl
 
 /--
 We then use the extracted graph to lower to ExprLow, which ensures the right
 ordering of instances.
 -/
-def mergeLhsLower := mergeLhsOrdered.fst.lower.get rfl
+def LhsLower := LhsOrdered.fst.lower.get rfl
 
-@[drunfold] def mergeRhs : ExprHigh String := [graph|
+@[drunfold] def Rhs : ExprHigh String := [graph|
     out0 [type = "io"];
+    out1 [type = "io"];
+    out2 [type = "io"];
     inp0 [type = "io"];
-    inp1 [type = "io"];
-    inp2 [type = "io"];
 
-    merge3 [type = "Merge3"];
+    fork3 [type = "Fork3"];
 
-    inp0 -> merge3 [inp = "inp0"];
-    inp1 -> merge3 [inp = "inp1"];
-    inp2 -> merge3 [inp = "inp2"];
+    inp0 -> fork3 [inp = "inp0"];
 
-    merge3 -> out0 [out = "out0"];
+    fork3 -> out0 [out = "out0"];
+    fork3 -> out1 [out = "out1"];
+    fork3 -> out2 [out = "out2"];
   ]
 
-def mergeRhsLower := mergeRhs.lower.get rfl
+def RhsLower := Rhs.lower.get rfl
 
 def rewrite : Rewrite String :=
   { pattern := matcher,
-    input_expr := mergeLhsLower,
-    output_expr := mergeRhsLower }
+    input_expr := LhsLower,
+    output_expr := RhsLower }
 
 namespace TestRewriter
 
-def mergeHigh : ExprHigh String :=
+def fullCircuit : ExprHigh String :=
   [graph|
     src0 [type="io"];
     snk0 [type="io"];
 
     fork1 [type="Fork"];
     fork2 [type="Fork"];
-    merge2 [type="Merge"];
-    merge1 [type="Merge"];
+    merge2 [type="merge"];
+    merge1 [type="merge"];
 
-    src0 -> fork1 [inp="out0"];
+    src0 -> fork1 [inp="inp0"];
 
-    fork1 -> fork2 [out="out0",inp="inp0"];
+    fork1 -> fork2 [out="out1",inp="inp0"];
 
-    fork1 -> merge1 [out="out1",inp="inp0"];
+    fork1 -> merge1 [out="out0",inp="inp0"];
     fork2 -> merge1 [out="out0",inp="inp1"];
     fork2 -> merge2 [out="out1",inp="inp1"];
 
@@ -108,8 +108,8 @@ def mergeHigh : ExprHigh String :=
     merge2 -> snk0 [out="out0"];
   ]
 
-#eval DataflowRewriter.rewrite "rw0_" mergeHigh rewrite |> toString |> IO.print
+#eval DataflowRewriter.rewrite "rw0_" fullCircuit rewrite |> toString |> IO.print
 
 end TestRewriter
 
-end DataflowRewriter.MergeRewrite
+end DataflowRewriter.ForkRewrite
